\documentclass[twocolumn, 11pt]{article}
\usepackage[utf8]{inputenc}
\usepackage[german,english]{babel}
\renewcommand{\baselinestretch}{1.05}
\usepackage{amsmath,amsthm,verbatim,amssymb,amsfonts,amscd, graphicx}
\usepackage{graphicx}
\usepackage{mhchem}
\newcommand{\R}{\mathbb{R}}
\newcommand{\Q}{\mathbb{Q}}
\newcommand{\C}{\mathbb{C}}
\newcommand{\N}{\mathbb{N}}
\renewcommand{\i}{\mathrm{i}}
\newcommand{\e}{\mathrm{e}}
\newcommand{\norm}[1]{\left\Vert #1 \right\Vert}
\newcommand{\abs}[1]{\left| #1 \right|}
\newcommand{\diam}{\mathrm{diam}}
\renewcommand{\d}[1]{\,d{#1}}
\newcommand{\dd}[2]{\frac{d{#1}}{d{#2}}}
\newcommand{\pd}[2]{\frac{\partial #1 }{\partial #2}}
\usepackage{braket}
\usepackage{booktabs}
\usepackage{enumerate}
\usepackage{siunitx}
\usepackage{floatrow}
\setlength{\columnseprule}{0.4pt}
\thispagestyle{empty}
%%% LENGTHS
\usepackage{geometry}
 \geometry{
 a4paper,
 left=10mm,
 top=10mm,
 right=10mm,
 bottom=10mm
 }

\begin{document}
%
\section*{Formulas for Quantum Optics}
\begin{description}
  \item[Displacement Operator]
\begin{align*}
  D(\alpha) = \e^{\alpha a^{\dagger} - \alpha ^{\ast} a} = \e^{- \frac{1}{2} \abs{\alpha}^2} \e^{\alpha a ^{\dagger}} \e^{- \alpha ^{\ast} a} && D(\alpha) \Ket{0} = \Ket{\alpha} \\
  D(\alpha) = D(-\alpha) \\
  D(\alpha) D(\beta) = \e^{\i \Im (\alpha \beta^{\ast})} D(\alpha + \beta)
\end{align*}
%
\item [Squeeze Operator] 
\begin{align*}
  S(\zeta) = \e^{\frac{1}{2} (\zeta {a^{\dagger}}^2 - \zeta^{\ast} a^2)} &&
 \zeta = r \e^{i \theta} \\
  \theta = 0 \implies \Delta X_1 ^2 = \frac{1}{4} e^{-2 r} &&  \Delta X_2 ^2 = \frac{1}{4} e^{2 r}
\end{align*}
%
%
\begin{align*}
  \Braket{\zeta | a ^{\dagger} a | \zeta} = \sinh^2 r && \\
  \Braket{\zeta | a | \zeta} = 0 && \\
  \Braket{\zeta | a^2 | \zeta} = -e ^{\i \varphi} \sinh r \cosh r && \\
  \Braket{\zeta | (a^{\dagger} a )^2 | \zeta} = 2 \cosh^2 r \sinh^2 r + \sinh^4 r
\end{align*}
%

\item[Properties of the Commutator] 
%
\begin{align*}
  [A, BC] &= [A, B] C + B [A, C] \\
  [BC, A] &= [B, A] C + B [C, A] \\
  [A, B] &= - [B, A]
\end{align*}
%
\item [Beam Splitter]
phase shift operator
%
\begin{align*}
  P(\phi) = \e^{- \i \phi \hat{n}}
\end{align*}
%
\begin{align*}
  a_0 & = \frac{a_2 - \i a_3}{\sqrt{2}} & a_1 & = \frac{a_3 - \i a_2}{\sqrt{2}} \\
  D_0(\alpha) & = D_2(\frac{\alpha}{\sqrt{2}}) D_3(\frac{- \i \alpha}{\sqrt{2}}) \\
  D_1(\alpha) & = D_3(\frac{\alpha}{\sqrt{2}}) D_2(\frac{\i \alpha}{\sqrt{2}})
\end{align*}
%
%
\item[Baker-Campbell Hausdorff Theorem] 
\begin{align*}
  & \e^{A + B}  = \e^A \e^B \e^{\frac{1}{2} [B, A]} = \e^B \e^A \e^{\frac{1}{2} [A, B]} \\
  \text{ falls } & [A, [A, B]] = [B, [A, B]] = 0
\end{align*}
%
  
\item[Baker-Campbell Hausdorff Lemma] 

\item[Number Operator] 
\item[Quantum Harmonic Oscillator] $ $\\
  Spread of Ground wave function $\sqrt{ \hbar /(m \omega)}$
    %
    %
    \begin{align*}
      E_x = E_0 (a + a^{\dagger}) \sin{k z} &&
      B_y = - \i B_0 (a - a^{\dagger}) \cos{k z}
    \end{align*}
    %
    \begin{align*}
      H = \hbar \omega \left(\hat{n} + \frac{1}{2}\right) =
      \frac{1}{2} \left( \frac{p}{m} + m \omega^2 q^2 \right) \\ a, a^{\dagger} = \frac{1}{\sqrt{2 \hbar m \omega}}(m \omega \hat{q} \pm \i p)
    \end{align*}
    %
    %
    \begin{align*}
      \hat{n} = a^{\dagger} a && \hat{n} \Ket{n} = n \Ket{n} && \Ket{n} = \frac{a^{\dagger n}}{\sqrt{n!}} \Ket{0}
    \end{align*}
    %
    %
    \begin{align*}
      a ^{\dagger} \Ket{n} &= \sqrt{n + 1} \Ket{ n + 1} & a \Ket{n} &= \sqrt{n} \Ket{n - 1} \\
      [a^{m}, a^{\dagger}] &= m a^{m-1} & [a, a^{\dagger m}] &= m (a^{\dagger})^{m-1}  \\
      [n, a^{m}] &= - m a^{m} & [n, a^{\dagger m}] &= m a^{\dagger m}
    \end{align*}
    %
\begin{align*}
  [a_i, a_j ^{\dagger}] = \delta_{ij} && [a_i, a_j] = [a_i^{\dagger}, a_j^{\dagger}] = 0
\end{align*}
%
  \item[Quadratures]
    %
    \begin{align*}
      X_1 = \frac{1}{2}\left( a + a^{\dagger} \right) \propto q &&
      X_2 = \frac{1}{2 \i}\left( a - a^{\dagger} \right) \propto p \\
    \end{align*}
    %
    
  \item[Phase State]
    %
    \begin{align*}
      P(\varphi) = \frac{1}{2 \pi} \abs{\Braket{\varphi | \psi} }^2  &&
    \Ket{\varphi} = \sum_{n=0}^{\infty} \e^{\i n \varphi} \Ket{n}
    \end{align*}
    %
    
  \item[Coherent States]
    %
    \begin{align*}
      \Ket{\alpha} = e^{- \abs{\alpha}^2 /2} \sum_{n}^{} \frac{\alpha^n}{\sqrt{n!}} \Ket{n} && \bar{n} = \abs{\alpha}^2 \\
      \Braket{\alpha | \beta} = \e^{\frac{1}{2} (\beta ^{\ast} \alpha - \beta \alpha^{\ast})}
      \e^{- \frac{1}{2} \abs{\beta - \alpha}^{2}} && a \Ket{\alpha} = \alpha \Ket{\alpha} 
    \end{align*}
    %
  \item[Characteristic Functions]
    %
    \begin{align*}
      & W(\alpha, \alpha ^{\ast}) = \frac{2}{\pi^2} \e^{2 \abs{\alpha}^2}
      \int \d{^2 \eta} \Braket{- \eta | \rho | \eta} \e^{-2 (\eta \alpha ^{\ast} - \eta^{\ast} \alpha)} \\
      & Q(\alpha, \alpha^{\ast}) = \frac{1}{\pi} \Braket{\alpha | \rho | \alpha}
    \end{align*}
    %
  \item [Correlation Functions]
    %
    \begin{align*}
      \hat{E}^+(\vec{r}, t) = \i \epsilon_0/2 a \e^{-\i (\omega t - \vec{k} \vec{r})}
      && \hat{E}^- = \hat{E^+} ^{\dagger}
    \end{align*}
    %
    \begin{align*}
      g^{(1)}(\tau) & = \frac{\Braket{E^-(t) E^+(t+\tau)}}{\Braket{E^-(t) E^+(t)}} \\
      g^{(2)}(\tau) & = \frac{\Braket{E^-(t) E^-(t + \tau) E^+(t + \tau) E^+(\tau) }}{\Braket{E^-(t) E^+(t)}^2}
    \end{align*}
    %
    %
    \begin{align*}
      Q = \Braket{\hat{n}} (g^{(2)}(0) - 1)
    \end{align*}
    %
  \item[Bloch Equations]
    %
    %
    \begin{align*}
      \sigma_+ = \Ket{e}\Bra{g} && \sigma_- = \Ket{g}\Bra{e} && \sigma_3 = \Ket{e}\Bra{e} - \Ket{g}\Bra{g}
    \end{align*}
    %
    
    \begin{align*}
      u = 2 \Re (\rho_{12}) && v = 2 \Im(\rho_{12}) && w = \rho_{11} - \rho_{22}
    \end{align*}
    %
    %
    \begin{align*}
      W = \Omega \vec{e}_1 + \Delta \vec{e}_3 \text{ Precession around this vector} \\
\Delta = \omega_L - \omega_0
    \end{align*}
    %
    
    %
    
\end{description}


\end{document}
